Add definitions for domains of substitution maps

LambdaGraph/Subst.lean
@@ -3,13 +3,15 @@ module
 import all LambdaGraph.SubstMaps
 public import LambdaGraph.Nest
 
+macro_rules | `(tactic| get_elem_tactic_extensible) => `(tactic| grind)
+
 @[grind]
 structure SubstProps (p p' : Program) (e e' : Expr) (vm : VarMap p.size)
     (fm : FunMap p.size) (fm' : FunMap p'.size) : Prop where
   pre : p.Prefix p'
   op : Termination.OccursProvenance p p' vm vm.extend fm fm'
   ep : Termination.ExprProvenance p p' e e' vm fm
-  ext : ∀ (m : Nat) hm, fm[m]'hm ≠ m → fm'[m]'(by grind) = fm[m]
+  ext : ∀ (m : Nat) hm, fm[m]'hm ≠ m → fm'[m] = fm[m]
 
 /--
 The result of a substitution.
@@ -39,7 +41,7 @@ no reason such a procedure could not be implemented).
 -/
 noncomputable def Expr.subst (p : Program) (e : Expr) (vm : VarMap p.size)
     (fm : FunMap p.size) : SubstResult p e vm fm :=
-  if ∀ n (_ : n < p.size), e.Free p n → vm[n] = var n then
+  if ∀ n, e.Free p n → ¬vm.Dom n then
     -- The expression does not contain a free substitution variable, so there is
     -- nothing to do.
     ⟨p, e, fm, by rfl, by simp, by simp, by simp⟩
@@ -49,7 +51,10 @@ noncomputable def Expr.subst (p : Program) (e : Expr) (vm : VarMap p.size)
       ⟨p, vm[m]?.getD (var m), fm, by rfl, by simp, by grind, by simp⟩
     | fn m =>
       if hm : m < p.size then
-        if hfmm : fm[m] = m then
+        if hfmm : fm.Dom m then
+          -- There is already a substitution for this function, we can reuse it.
+          ⟨p, fn fm[m], fm, by rfl, by simp, by grind, by simp⟩
+        else
           -- There is not yet a substitution for this function, so we have to
           -- create a new one.
           let m' := p.size
@@ -60,7 +65,7 @@ noncomputable def Expr.subst (p : Program) (e : Expr) (vm : VarMap p.size)
           -- Substitute the body to obtain the body for the new function.
           let ⟨p₂, f', fm₂, h⟩ := p.fn[m].subst p₁ vm₁ fm₁
           -- Now put the final function body in place.
-          let p₃ := p₂.setBody m' f' (hi := by grind)
+          let p₃ := p₂.setBody m' f'
           let e' := fn m'
           ⟨p₃, e', fm₂, by
             refine ⟨?_, ?_, ?_, ?_⟩
@@ -69,11 +74,8 @@ noncomputable def Expr.subst (p : Program) (e : Expr) (vm : VarMap p.size)
                 grind [Occurs, OccursProvenance, Program.UsesFn]
               grind [Occurs, OccursProvenance, Program.UsesFn]
             · grind [ExprProvenance]
-            · grind
+            · grind [FunMap.Dom]
           ⟩
-        else
-          -- There is already a substitution for this function, we can reuse it.
-          ⟨p, fn fm[m], fm, by rfl, by simp, by grind, by simp⟩
       else
         -- This case is actually impossible, nonexistent functions don't have
         -- free variables.
@@ -105,7 +107,7 @@ decreasing_by
       intro n h
       grind [Reachable.there]
     have hm₁ : m ∉ reachableUnmapped p₁ (fn m) fm₁ := by grind
-    have hm₂ : m ∈ reachableUnmapped p (fn m) fm := by grind
+    have hm₂ : m ∈ reachableUnmapped p (fn m) fm := by grind [FunMap.Dom]
     grind
   all_goals grind
 
@@ -149,19 +151,19 @@ theorem Expr.subst_types {p : Program} {e : Expr} {t : Ty} {vm : VarMap p.size}
       have .var _ _ := ht
       apply hvm
     · simp [hm, ht]
+  next p vm fm m hm hfmm hf =>
+    have .fn _ _ := ht
+    obtain ⟨_, hty, hret⟩ := hfm _ ‹m < p.size›
+    rw [hty, hret]
+    constructor
   next p vm fm m hm hfmm m' vm₁ fm₁ p₁ p₂ f' fm₂ h₂ hs₂ p₃ f'' hf ih =>
     rw [hs₂] at ih
     dsimp only at ih
     have .fn _ _ := ht
     have hp₂ : p₂ = (p.fn[m].subst p₁ vm₁ fm₁).program := by grind
     subst hp₂
-    have hty : p.ty[m] = p₃.ty[p.size]'(by grind) := by grind [Program.prefix_subst.ty_eq]
-    have hret : p.ret[m] = p₃.ret[p.size]'(by grind) := by grind [Program.prefix_subst.ret_eq]
-    rw [hty, hret]
-    constructor
-  next p vm fm m hm hfmm hf =>
-    have .fn _ _ := ht
-    obtain ⟨_, hty, hret⟩ := hfm _ ‹m < p.size›
+    have hty : p.ty[m] = p₃.ty[p.size] := by grind [Program.prefix_subst.ty_eq]
+    have hret : p.ret[m] = p₃.ret[p.size] := by grind [Program.prefix_subst.ret_eq]
     rw [hty, hret]
     constructor
   next => exact ht
@@ -230,7 +232,10 @@ theorem FunMap.Original.lt {n : Nat} {fm : FunMap n} {m : Nat}
 
 @[grind →]
 theorem FunMap.Original.map {n : Nat} {fm : FunMap n} {m : Nat}
-    (hm : m < n) (h : fm.Original fm[m]) : fm[m] = m := h.2 hm rfl
+    (hm : m < n) (h : fm.Original fm[m]) : ¬fm.Dom m := by
+  rintro ⟨_, hne⟩
+  have := h.2 hm rfl
+  contradiction
 
 theorem FunMap.original_update {n : Nat} {fm : FunMap n} {m k : Nat}
     (hm : m < n) (h : fm.Original k) : (fm.update m hm).Original k := by
@@ -381,19 +386,23 @@ theorem Expr.deepOriginal_mk {p : Program} {e : Expr} (hp : p.ValidRefs)
 
 def FunMap.LocalProvenance {n : Nat} (fm : FunMap n) (e e' : Expr) (k : Option Nat) :
     Prop :=
-  ∀ ⦃m r⦄ (_ : m < n), fm[m] ≠ m → e'.Local fm[m] r → m = k ∨ e.Local m r
+  ∀ ⦃m r⦄ (hm : fm.Dom m), e'.Local fm[m] r → m = k ∨ e.Local m r
 
 structure FunMap.Valid {n : Nat} (fm : FunMap n) : Prop where
   lt : ∀ {m} (_ : m < n), fm[m] < n
-  inj : ∀ {m k} (_ : m < n) (_ : k < n),
-    fm[m] ≠ m → fm[k] ≠ k → fm[m] = fm[k] → m = k
-  idem : ∀ {m} (_ : m < n), (fm[fm[m]]'(lt _)) = fm[m]
+  inj : ∀ {m k} (hm : fm.Dom m) (hk : fm.Dom k), fm[m] = fm[k] → m = k
+  idem : ∀ {m} (_ : m < n), fm[fm[m]] = fm[m]
 
 grind_pattern FunMap.Valid.lt =>
   fm.Valid, m < n, fm[m]
   where m =/= fm[_]'_
 
 attribute [grind =] FunMap.Valid.idem
+
+theorem FunMap.Valid.not_dom_map {n : Nat} {fm : FunMap n} (h : fm.Valid)
+    {m : Nat} (hm : m < n) : ¬fm.Dom fm[m] := by
+  rintro ⟨_, hne⟩
+  exact hne (h.idem hm)
 
 theorem FunMap.valid_mk {n : Nat} : (mk n).Valid := by
   constructor <;> grind
@@ -408,12 +417,7 @@ theorem FunMap.valid_update {n : Nat} {fm : FunMap n} {i : Nat}
     · simp [*]
     · replace hk : k < n := by lia
       grind
-  case inj =>
-    intro m k hm hk hmm' hkk' heq
-    replace hm : m < n := by grind
-    replace hk : k < n := by grind
-    have := h.inj hm hk
-    grind
+  case inj => grind [h.inj]
   case idem =>
     intro m hm
     by_cases m = n
@@ -425,12 +429,25 @@ theorem FunMap.valid_update {n : Nat} {fm : FunMap n} {i : Nat}
 structure FunMap.Extends {n' n : Nat} (fm' : FunMap n') (fm : FunMap n) : Prop where
   valid : fm'.Valid
   le : n ≤ n'
-  eq : ∀ {m} (_ : m < n), fm[m] ≠ m → fm'[m] = fm[m]
+  eq : ∀ {m} (hm : fm.Dom m), fm'[m] = fm[m]
   eq_of_lt : ∀ {m} (_ : m < n'), fm'[m] < n → ∃ (_ : m < n), fm'[m] = fm[m]
   exists_of_ge : ∀ {m'}, n ≤ m' → m' < n' → ∃ (m : Nat) (_ : m < n), fm'[m] = m'
 
 grind_pattern FunMap.Extends.eq =>
-  fm'.Extends fm, fm[m], fm'[m]
+  fm'.Extends fm, fm.Dom m, fm'[m]
+
+@[grind →]
+theorem FunMap.dom_of_extends {n n' : Nat} {fm : FunMap n} {fm' : FunMap n'}
+    {m : Nat} (hext : fm'.Extends fm) (h : fm.Dom m) : fm'.Dom m := by
+  have := hext.eq h
+  grind [Dom]
+
+@[grind →]
+theorem FunMap.dom_of_extends_of_lt {n n' : Nat} {fm : FunMap n}
+    {fm' : FunMap n'} {m : Nat} (hext : fm'.Extends fm) (h : fm'.Dom m)
+    (hlt : fm'[m] < n) : fm.Dom m := by
+  have := hext.eq_of_lt h.1 hlt
+  grind [Dom]
 
 theorem FunMap.extends_self {n : Nat} {fm : FunMap n} (hfm : fm.Valid) :
     fm.Extends fm := by constructor <;> grind
@@ -439,6 +456,7 @@ theorem FunMap.extends_self {n : Nat} {fm : FunMap n} (hfm : fm.Valid) :
 theorem FunMap.extends_trans {n₀ n₁ n₂ : Nat} {fm₀ : FunMap n₀}
     {fm₁ : FunMap n₁} {fm₂ : FunMap n₂} (h : fm₁.Extends fm₀)
     (h' : fm₂.Extends fm₁) : fm₂.Extends fm₀ := by
+  have : ∀ m, fm₀.Dom m → fm₁.Dom m := fun m => dom_of_extends h
   obtain ⟨hfm₁, hle, h₀, h₁, h₂⟩ := h
   obtain ⟨hfm₂, hle', h₀', h₁', h₂'⟩ := h'
   constructor
@@ -451,6 +469,7 @@ theorem FunMap.extends_trans {n₀ n₁ n₂ : Nat} {fm₀ : FunMap n₀}
   · intro m' hge hlt
     by_cases h : m' < n₁
     · obtain ⟨m, hm, hfmm⟩ := h₂ hge h
+      have : fm₁.Dom m := ⟨by lia, by grind⟩
       exact ⟨m, hm, by grind⟩
     · simp only [Nat.not_lt] at h
       obtain ⟨m, hm, hfmm⟩ := h₂' h hlt
@@ -458,16 +477,14 @@ theorem FunMap.extends_trans {n₀ n₁ n₂ : Nat} {fm₀ : FunMap n₀}
       · exact ⟨m, h, hfmm⟩
       · simp only [Nat.not_lt] at h
         obtain ⟨k, hk, hfmk⟩ := h₂ h hm
-        have heq := h₀' (show k < n₁ by lia) (by grind)
-        have := hfm₂.idem (show k < n₂ by lia)
-        simp [heq, hfmk] at this
-        grind
+        have : fm₁.Dom k := ⟨by lia, by grind⟩
+        exact ⟨k, hk, by grind⟩
   · grind
 
 theorem FunMap.extends_update {n : Nat} {fm : FunMap n} {m : Nat} (hm : m < n)
-    (hfm : fm.Valid) (h : fm.Original m) (hfmm : fm[m] = m) :
+    (hfm : fm.Valid) (h : fm.Original m) (hfmm : ¬fm.Dom m) :
     (fm.update m hm).Extends fm := by
-  constructor <;> grind [valid_update]
+  constructor <;> grind [Dom, valid_update]
 
 grind_pattern FunMap.extends_update => fm.Original m, fm.update m hm
 
@@ -544,16 +561,15 @@ grind_pattern FunMap.valid_subst => (e.subst p vm fm).funMap
 
 structure VarMap.Valid {n : Nat} (vm : VarMap n) (fm : FunMap n) : Prop where
   bounded : ∀ {m} (_ : m < n), vm[m].Bounded n
-  localProvenance : ∀ {m} (_ : m < n),
-    fm[m] ≠ m → fm.LocalProvenance (.var m) vm[m] none
-  original : ∀ {m} (_ : m < n),
-    fm[m] = m → vm[m] ≠ .var m → vm[m].Original fm
+  localProvenance : ∀ {m} (hm : fm.Dom m),
+    fm.LocalProvenance (.var m) vm[m] none
+  original : ∀ {m} (hm : vm.Dom m), ¬fm.Dom m → vm[m].Original fm
 
 attribute [grind! .] VarMap.Valid.bounded
 
 theorem VarMap.valid_mk {n m : Nat} {v : Expr} (hv : v.Bounded n) :
     (mk n m v).Valid (.mk n) := by
-  constructor <;> grind [Expr.original_mk]
+  constructor <;> grind [FunMap.Dom, Expr.original_mk]
 
 theorem VarMap.valid_update {p : Program} {vm : VarMap p.size}
     {fm : FunMap p.size} {i : Nat} (hi : i < p.size) (hvm : vm.Valid fm)
@@ -569,22 +585,14 @@ theorem VarMap.valid_update {p : Program} {vm : VarMap p.size}
       · replace hk : k < p.size := by lia
         simpa [*] using Expr.bounded_of_ge (by lia) (hvm.bounded hk)
   case localProvenance =>
-    intro m hm hmm' n r hn hnn' hl
-    have : m ≠ p.size := by
-      intro rfl
-      simp at hmm'
-    replace hm : m < p.size := by lia
-    have : n ≠ p.size := by
-      intro rfl
-      simp at hnn'
-    replace hn : n < p.size := by lia
+    intro m hfmm n r hfmn hl
+    have hm : m < p.size := by grind
+    have hn : n < p.size := by grind
     by_cases i = m
     · grind
     · have : i ≠ n := by grind
-      apply hvm.localProvenance <;> simp_all
-  case original =>
-    intro m hm hmm' hne
-    grind [Expr.original_update, hvm.original]
+      apply hvm.localProvenance <;> grind
+  case original => grind [Expr.original_update, hvm.original]
 
 theorem VarMap.valid_subst {p : Program} {e : Expr} {vm : VarMap p.size}
     {fm : FunMap p.size} (hvm : vm.Valid fm) (hfm : fm.Valid)
@@ -608,27 +616,30 @@ theorem VarMap.valid_subst {p : Program} {e : Expr} {vm : VarMap p.size}
     constructor
     case bounded => grind
     case localProvenance =>
-      intro k hk hkk' l r hl hll' hlc
-      by_cases k < p.size
+      intro k hfmk l r hfml hlc
+      by_cases hk : k < p.size
       · simp only [VarMap.getElem_extend_lt, *] at hlc
-        by_cases m = k
+        by_cases hmk : m = k
         · subst k
           have hl' : fm₂[l] < p.size := hvm.bounded hm hlc
-          obtain ⟨hl, heq⟩ := hext.eq_of_lt hl hl'
+          obtain ⟨hl, heq⟩ := hext.eq_of_lt hfml.1 hl'
           rw [heq] at hlc
-          by_cases hvmm : vm[m] = .var m
-          · grind
-          · grind [hvm.original hm (by simp [*]) hvmm hlc]
-        · exact hvm₂.localProvenance hk hkk' hl hll' (by grind)
-      · exact hvm₂.localProvenance hk hkk' hl hll' (by grind)
+          by_cases hvmm : vm.Dom m
+          · grind [hvm.original hvmm hfmm hlc]
+          · grind [Dom]
+        · apply hvm₂.localProvenance hfmk hfml
+          simp [vm₁, show k < p.size + 1 by lia, *]
+      · apply hvm₂.localProvenance hfmk hfml
+        simp only [Nat.not_lt] at hk
+        simpa [vm₁, show p.size + 1 ≤ k by grind, *] using hlc
     case original =>
-      intro k hk hkk' hne
-      dsimp only at hk hkk'
+      intro k hvmk hfmk
+      dsimp only at hfmk
       by_cases hk : k < p.size
-      · have hkk' : fm[k] = k := by grind
-        simp only [getElem_extend_lt, *] at hne ⊢
-        exact Expr.original_of_extends hext (hvm.original hk hkk' hne)
-      · simp_all
+      · replace hfmk : ¬fm.Dom k := by grind
+        simp only [getElem_extend_lt, hk]
+        exact Expr.original_of_extends hext (hvm.original (by grind) hfmk)
+      · grind
 
 grind_pattern VarMap.valid_subst =>
   vm.extend (n' := (e.subst p vm fm).program.size)
@@ -647,20 +658,20 @@ theorem Expr.localProvenance_subst {p : Program} {e : Expr} {vm : VarMap p.size}
     fm'.LocalProvenance e e' none := by
   fun_induction Expr.subst
   next p e vm fm h =>
-    intro n r hn hnn' hl
+    intro n r hn hl
     have := (ho.1 hl).map
     contradiction
   next p vm fm m h =>
-    intro n r hn hnn' hl
+    intro n r hn hl
     have hm : m < p.size := by grind
     simp only [hm, getElem?_pos, Option.getD_some] at hl
-    by_cases hmm' : fm[m] = m
-    · simp only [Classical.not_forall] at h
-      obtain ⟨k, hk, hf, hne⟩ := h
-      have .var := hf
-      have := hvm.original hm hmm' hne hl
-      grind
-    · exact hvm.localProvenance hm hmm' hn hnn' hl
+    by_cases hfmm : fm.Dom m
+    · exact hvm.localProvenance hfmm hn hl
+    · simp only [free_in_var_iff, forall_eq, Classical.not_not] at h
+      grind [hvm.original h hfmm hl]
+  next p vm fm m hm hfmm hf =>
+    intro n r hfmn hl
+    grind [hfm.inj]
   next p vm fm m hm hfmm m' vm₁ fm₁ p₁ p₂ f' fm₂ h₂ hs₂ p₃ e' hf ih =>
     rw [hs₂] at ih
     dsimp only at ih ⊢
@@ -668,17 +679,13 @@ theorem Expr.localProvenance_subst {p : Program} {e : Expr} {vm : VarMap p.size}
     have hfm₁ : fm₁.Valid := FunMap.valid_update hm (by grind) hfm
     have hext₂ : fm₂.Extends fm₁ := by grind
     have hfm₂ : fm₂.Valid := hext₂.valid
-    intro n r hn hnn' hl
+    intro n r hfmn hl
     subst e'
     simp only [local_fn_iff] at hl
     obtain ⟨hr, hmn'⟩ := hl
-    have : fm₂[m]'(by grind) = m' := by grind
+    have : fm₂[m] = m' := by grind
     rw [← this] at hmn'
-    have : m = n := hfm₂.inj (by grind) hn (by grind) hnn' hmn'
-    simp [*]
-  next p vm fm m hm hfmm hf =>
-    intro n r hn hnn' hl
-    grind [hfm.inj]
+    grind [hfm₂.inj (by grind) hfmn hmn']
   next => grind
   next p vm fm b h => simp [FunMap.LocalProvenance]
   next p vm fm k e₁ e₂ p₁ e₁' fm₁ h₁ hs₁ p₂ e₂' fm₂ h₂ hs₂ h ih₁ ih₂ =>
@@ -690,15 +697,16 @@ theorem Expr.localProvenance_subst {p : Program} {e : Expr} {vm : VarMap p.size}
     obtain ⟨ho₁, ho₂⟩ := Expr.deepOriginal_bin_iff.mp ho
     have hf' := ih₁ hvm hfm ho₁
     have he' := ih₂ hvm₁ hfm₁ (deepOriginal_of_extends (by grind) (by grind) ho₂)
-    intro n r hn hnn' hl
+    intro n r hfmn hl
     have hext₁ : fm₂.Extends fm₁ := by grind
     have hv₁' : e₁'.ValidRefs p₁ := by grind [validRefs_subst]
     obtain hl | hl := Expr.local_bin_iff.mp hl
-    · replace ⟨hn, heq⟩ := hext₁.eq_of_lt hn (hv₁' hl)
+    · replace ⟨hn, heq⟩ := hext₁.eq_of_lt hfmn.1 (hv₁' hl)
       rw [heq] at hl
-      have := hf' hn (by grind) hl
+      replace hfmn : fm₁.Dom n := by grind
+      have := hf' hfmn hl
       grind
-    · have := he' hn hnn' hl
+    · have := he' hfmn hl
       grind
   next p vm fm c et ef p₁ c' fm₁ h₁ hs₁ vm₁ p₂ et' fm₂ h₂ hs₂ p₃ ef' fm₃ h₃ hs₃
       hf ihc ihet ihef =>
@@ -716,27 +724,27 @@ theorem Expr.localProvenance_subst {p : Program} {e : Expr} {vm : VarMap p.size}
       (deepOriginal_of_extends (by grind) (by grind) hoet)
     have hef' := ihef hvm₂ hfm₂
       (deepOriginal_of_extends (by grind) (by grind) hoef)
-    intro n r hn hnn' hl
+    intro n r hfmn hl
     have hext₁ : fm₃.Extends fm₁ := by grind
     have hext₂ : fm₃.Extends fm₂ := by grind
     have hvc' : c'.ValidRefs p₁ := by grind [validRefs_subst]
     have hvet' : et'.ValidRefs p₂ := by
       grind [validRefs_subst]
     obtain hl | hl | hl := Expr.local_cond_iff.mp hl
-    · replace ⟨hn, heq⟩ := hext₁.eq_of_lt hn (hvc' hl)
+    · replace ⟨hn, heq⟩ := hext₁.eq_of_lt hfmn.1 (hvc' hl)
       rw [heq] at hl
-      have := hc' hn (by lia) hl
+      have := hc' (by grind) hl
       grind
-    · replace ⟨hn, heq⟩ := hext₂.eq_of_lt hn (hvet' hl)
+    · replace ⟨hn, heq⟩ := hext₂.eq_of_lt hfmn.1 (hvet' hl)
       rw [heq] at hl
-      have := het' hn (by lia) hl
+      have := het' (by grind [FunMap.Dom]) hl
       grind
-    · have := hef' hn hnn' hl
+    · have := hef' hfmn hl
       grind
   next p vm fm e i p' e' fm' h hs hf ih =>
     rw [hs] at ih
     dsimp only at ih ⊢
-    intro n r hn hnn' hl
+    intro n r hfmn hl
     rw [Expr.local_proj_iff] at hl ⊢
     apply ih hvm hfm <;> grind
 
@@ -757,87 +765,41 @@ theorem Program.validRefs_subst {p : Program} {e : Expr} {vm : VarMap p.size}
   next => grind
 
 structure Program.ValidSubst (p : Program) (vm : VarMap p.size) (fm : FunMap p.size) where
-  fn_localProvenance : ∀ {m m'} (_ : m < p.size) (_ : m' < p.size),
-    m' = fm[m] → m' ≠ m → fm.LocalProvenance p.fn[m] p.fn[m'] m
-  eq_of_not_nests : ∀ {m} (_ : m < p.size),
-    (∀ n (_ : n < p.size), vm[n] ≠ .var n → n ⊁[p] m) → fm[m] = m
-  new_subst_var : ∀ {n m} (_ : n < p.size) (_ : m < p.size),
-    vm[n] ≠ .var n → n ≻[p] m → fm[m] = m → vm[m] = .var m
-  compat : ∀ {m} (_ : m < p.size), -- TODO Move to VarMap instead of localProvenance?
-    fm[m] ≠ m → vm[m] = .var m ∨ vm[m] = .var fm[m]
+  fn_localProvenance : ∀ {m} (hm : fm.Dom m) (hm' : fm[m] < p.size),
+    fm.LocalProvenance p.fn[m] p.fn[fm[m]] m
+  nests_of_dom : ∀ {m}, fm.Dom m → ∃ n, vm.Dom n ∧ n ≻[p] m
+  dom_of_nests : ∀ {n m}, vm.Dom n → n ≻[p] m → vm.Dom m → fm.Dom m
+  compat : ∀ {m} (hm : fm.Dom m), vm.Dom m → vm[m] = .var fm[m]
 
 theorem Program.validSubst_mk {p : Program} {n : Nat} {v : Expr} (hwf : p.WF) :
     p.ValidSubst (.mk _ n v) (.mk _) := by
-  constructor <;> grind [WF]
+  constructor <;> grind [VarMap.Dom, FunMap.Dom, WF]
 
 theorem Program.validSubst_push_recurse {p : Program} {vm : VarMap p.size}
-    {fm : FunMap p.size} {l i : Nat} (hl : l < p.size) (hi : i < p.size)
-    (hfm : fm.Valid) (hp : p.ValidRefs) (hvml : vm[l] ≠ .var l)
-    (hnestsi : l ≻[p] i) (hvalid : p.ValidSubst vm fm) :
+    {fm : FunMap p.size} {l i : Nat} (hi : i < p.size) (hfm : fm.Valid)
+    (hp : p.ValidRefs) (hvml : vm.Dom l) (hnestsi : l ≻[p] i)
+    (hvalid : p.ValidSubst vm fm) :
     (p.push (.recurse p.size) p.ty[i] p.ret[i]).ValidSubst
       (vm.update i hi) (fm.update i hi) := by
   constructor
   case fn_localProvenance =>
-    intro m m' hm hm' hfmm hmm' n r hn hnn' hl
+    intro m hfmm hm' n r hfmn hl
     by_cases hnm : n = m
     · simp [*]
     · right
-      have : m ≠ p.size := by
-        rintro rfl
-        simp [*] at hmm'
-      have : n ≠ p.size := by
-        rintro rfl
-        simp at hnn'
-      replace hm : m < p.size := by lia
-      replace hn : n < p.size := by lia
+      replace hm : m < p.size := by grind
+      replace hn : n < p.size := by grind
       have hm' := hfm.lt hm
       have hn' := hfm.lt hn
       have him : i ≠ m := by grind
       have hin : i ≠ n := by grind
-      simp only [ne_eq, not_false_eq_true, FunMap.getElem_update_ne, Vector.getElem_push_lt, hm,
-        him, hn, hin, hfmm, hm'] at hmm' hnn' hl
-      have := hvalid.fn_localProvenance hm hm' rfl hmm' hn hnn' hl
-      simp_all
-  case eq_of_not_nests =>
-    intro m hm h
-    by_cases m = p.size
-    · simp [*] at *
-    · replace hm : m < p.size := by lia
-      by_cases i = m
-      · grind
-      · rw [FunMap.getElem_update_ne hi hm ‹i ≠ m›]
-        apply hvalid.eq_of_not_nests
-        intro n hn hne
-        have := h n (by lia) (by grind)
-        grind
-  case new_subst_var =>
-    intro n m hn hm hvmn hnests hfmm
-    by_cases m = p.size
-    · simp [*]
-    · replace hm : m < p.size := by lia
-      by_cases i = m
-      · simp only [FunMap.getElem_update_eq, *] at hfmm
-        lia
-      · simp only [ne_eq, not_false_eq_true, FunMap.getElem_update_ne,
-          VarMap.getElem_update_ne, *] at hfmm ⊢
-        replace hnests : n ≻[p] m := by grind
-        replace hn : n < p.size := by grind
-        by_cases i = n
-        · subst n
-          exact hvalid.new_subst_var hl hm hvml (.trans _ _ _ hnestsi hnests) hfmm
-        · simp only [ne_eq, not_false_eq_true, VarMap.getElem_update_ne, *] at hvmn
-          exact hvalid.new_subst_var hn hm hvmn hnests hfmm
-  case compat =>
-    intro m hm hmm'
-    have : m ≠ p.size := by
-      intro rfl
-      simp at hmm'
-    replace hm : m < p.size := by lia
-    by_cases i = m
-    · simp [*]
-    · rw [FunMap.getElem_update_ne hi hm ‹_›] at hmm' ⊢
-      rw [VarMap.getElem_update_ne hi hm ‹_›]
-      cases hvalid.compat hm hmm' <;> simp [*]
+      replace hfmm : fm.Dom m := by grind
+      replace hfmn : fm.Dom n := by grind
+      have := hvalid.fn_localProvenance hfmm hm' hfmn (by simpa [*] using hl)
+      simpa [*]
+  case nests_of_dom => grind [hvalid.nests_of_dom]
+  case dom_of_nests => grind [hvalid.dom_of_nests]
+  case compat => grind [hvalid.compat]
 
 theorem Program.validSubst_subst {p : Program} {e : Expr} {vm : VarMap p.size}
     {fm : FunMap p.size} (hvm : vm.Valid fm) (hfm : fm.Valid) (hp : p.ValidRefs)
@@ -848,11 +810,11 @@ theorem Program.validSubst_subst {p : Program} {e : Expr} {vm : VarMap p.size}
   next p vm fm m hm hfmm m' vm₁ fm₁ p₁ p₂ f' fm₂ h₂ hs₂ p₃ e' hf ih =>
     rw [hs₂] at ih
     dsimp only at ih
-    simp only [Classical.not_forall] at hf
-    obtain ⟨l, hl, hf, hvml⟩ := hf
+    simp only [Classical.not_forall, Classical.not_not] at hf
+    obtain ⟨l, hf, hvml⟩ := hf
     have hnestsm : l ≻[p] m := by
       replace .fn _ hm hne hf := hf
-      exact .free _ _ hl hm hne hf
+      exact .free _ _ hvml.1 hm hne hf
     have hext₁ : fm₁.Extends fm := FunMap.extends_update hm hfm (by grind) hfmm
     have hvm₁ : vm₁.Valid fm₁ := VarMap.valid_update hm hvm hfm
     have hfm₁ : fm₁.Valid := hext₁.valid
@@ -860,71 +822,63 @@ theorem Program.validSubst_subst {p : Program} {e : Expr} {vm : VarMap p.size}
     have hvm₂ : vm₁.extend.Valid fm₂ := by grind [VarMap.valid_subst]
     have hfm₂ : fm₂.Valid := by grind
     have hvalid₂ := ih hvm₁ hfm₁ (validRefs_push hp (by grind))
-      (validSubst_push_recurse hl hm hfm hp hvml hnestsm hvalid) (by grind)
-    have hvmm : vm[m] = .var m :=
-      hvalid.new_subst_var hl hm hvml hnestsm (by simp [hfmm])
+      (validSubst_push_recurse hm hfm hp hvml hnestsm hvalid) (by grind)
     have hext := FunMap.extends_trans hext₁ hext₂
     have hprov : fm₂.LocalProvenance p.fn[m] f' none := by
-      grind [Expr.localProvenance_subst, ⇐ Expr.bounded_of_ge]
-    have hp₃ : p₃ = ((Expr.fn m).subst p vm fm).program := by
-      grind [Expr.subst]
-    have hpre : p.Prefix p₃ := hp₃ ▸ prefix_subst
+      grind [Expr.localProvenance_subst]
+    have hpre : p.Prefix p₃ := by grind
     constructor
     case fn_localProvenance =>
-      intro n n' hn hn' hfmn hnn' k r hk hkk' hl
-      subst n'
-      have hfmm : fm₂[m]'(by grind) = m' := by grind [hext₂.eq]
+      intro n hfmn hn' k r hfmk hl
+      have hfmm : fm₂[m] = m' := by grind [hext₂.eq]
       by_cases hnm : m = n
       · subst n
         simp only [Vector.getElem_set_self, p₃, hfmm] at hl
-        replace hl := hprov hk hkk' hl
+        replace hl := hprov hfmk hl
         simp only [reduceCtorEq, false_or] at hl
-        rw [hfmm] at hnn'
         have heq : p₂.fn[m] = p.fn[m] := by
           have hp₂ : p₂ = (p.fn[m].subst p₁ vm₁ fm₁).program := by grind
           subst p₂
           rw [prefix_subst.fn_eq (by lia)]
           simp [p₁, hm]
-        simp [p₃, *]
+        simp [p₃, hfmm ▸ hfmn.2, *]
       · have hnm' : fm₂[n] ≠ m' := by
           intro heq
           rw [← heq] at hfmm
-          have := hfm₂.inj (by lia) hn (by lia) (by grind) hfmm
+          have := hfm₂.inj (by grind) (by grind) hfmm
           contradiction
         simp only [ne_eq, not_false_eq_true, Ne.symm, Vector.getElem_set_ne, p₃, hnm'] at hl
         have hne : m' ≠ n := by grind
-        cases hvalid₂.fn_localProvenance hn hn' rfl hnn' hk hkk' hl <;> simp [p₃, *]
-    case eq_of_not_nests =>
+        cases hvalid₂.fn_localProvenance hfmn hn' hfmk hl <;> simp [p₃, *]
+    case nests_of_dom =>
       have hnestsm₃ : l ≻[p₃] m := by grind
-      intro n hn h
+      intro n hfmn
       by_cases m = n
       · subst n
-        exfalso
-        exact h l (by grind) (by simpa [hl] using hvml) hnestsm₃
-      · apply hvalid₂.eq_of_not_nests
-        intro k hk hne hnests
-        have hb : p₂.fn[m']'(by grind) = Expr.recurse m' := by -- TODO Remove?
+        grind
+      · obtain ⟨k, hvmk, hnests⟩ := hvalid₂.nests_of_dom hfmn
+        have hb : p₂.fn[m'] = Expr.recurse m' := by
           have hp₂ : p₂ = (p.fn[m].subst p₁ vm₁ fm₁).program := by grind
           subst p₂
           rw [prefix_subst.fn_eq (by lia)]
           grind
         replace hnests : k ≻[p₃] n := nests_in_setBody (by grind) (by grind) hnests
         grind
-    case new_subst_var =>
-      intro n k hn hk hvmn hnests hfmk
+    case dom_of_nests =>
+      intro n k hvmn hnests hvmk
       by_cases hk : k < p.size
-      · replace hfmk : fm[k] = k := by grind
-        replace hnests : n ≻[p] k := by grind
-        have hvmk := hvalid.new_subst_var (by grind) ‹_› (by grind) hnests hfmk
+      · replace hnests : n ≻[p] k := by grind
+        have := hvalid.dom_of_nests (by grind) hnests (by grind)
         grind
-      · simp only [Nat.not_lt] at hk
-        simp [*]
+      · grind
     case compat =>
-      intro k hk hkk'
-      cases hvalid₂.compat hk hkk' -- TODO Simplify?
-      · by_cases hk : k < p₁.size
-        · grind
-        · grind
+      intro k hfmk hvmk
+      have hfmm : ¬fm.Dom m := by grind
+      have := hvalid₂.compat hfmk (by grind)
+      by_cases m = k
+      · subst k
+        have := hvalid.dom_of_nests hvml hnestsm (by grind)
+        contradiction
       · grind
   next => grind [validRefs_subst]
   next => grind [validRefs_subst]
@@ -933,9 +887,8 @@ theorem Program.validSubst_subst {p : Program} {e : Expr} {vm : VarMap p.size}
 theorem Program.exists_of_ge_in_subst {p : Program} {e : Expr}
     {vm : VarMap p.size} {fm : FunMap p.size} (hfm : fm.Valid)
     (ho : e.DeepOriginal p fm) {n' : Nat} (hn' : p.size ≤ n') :
-    let ⟨p', _, fm', h⟩ := e.subst p vm fm
-    let hsize := h.pre.size_le
-    n' < p'.size → ∃ (n : Nat) (_ : n < p.size), fm'[n] = n' := by
+    let ⟨p', _, fm', _⟩ := e.subst p vm fm
+    n' < p'.size → ∃ (n : Nat) (hn : n < p.size), fm'[n] = n' := by
   intro hlt
   have hext : (e.subst p vm fm).funMap.Extends fm := FunMap.extends_subst hfm ho
   obtain ⟨n, hn, hfmn⟩ := hext.exists_of_ge hn' hlt
@@ -946,8 +899,7 @@ theorem Program.pathWithout_of_pathWithout_in_subst_of_ge {p : Program}
     (hfm : fm.Valid) (hp : p.ValidRefs) (hvalid : p.ValidSubst vm fm)
     (ho : e.DeepOriginal p fm) {n' m' k' : Nat} (hn' : p.size ≤ n')
     (hm' : p.size ≤ m') (hk' : p.size ≤ k') :
-    let ⟨p', _, fm', h⟩ := e.subst p vm fm
-    let hsize := h.pre.size_le
+    let ⟨p', _, fm', _⟩ := e.subst p vm fm
     n' < p'.size → m' < p'.size → k' < p'.size → m' ⟶[p', n']* k' →
       ∃ (n m k : Nat) (hn : n < p.size) (hm : m < p.size) (hk : k < p.size),
         fm'[n] = n' ∧ fm'[m] = m' ∧ fm'[k] = k' ∧ m ⟶[p, n]* k := by
@@ -964,19 +916,20 @@ theorem Program.pathWithout_of_pathWithout_in_subst_of_ge {p : Program}
     have hne : n ≠ m := by grind
     exact ⟨n, m, m, hn, hm, hm, hfmn, hfmm, hfmm, .refl _ hne⟩
   | step m' l' k' hne' hs' hp' ih =>
-    obtain ⟨m, hm, hfmm⟩ := exists_of_ge_in_subst hfm ho hm' hmlt
+    obtain ⟨m, hm, hmm'⟩ := exists_of_ge_in_subst hfm ho hm' hmlt
     have hl' : p.size ≤ l' := by grind
     obtain ⟨_, hlf'⟩ := hs'
     have hllt : l' < p'.size := by grind
-    have ⟨n, l, k, hn, hl, hk, hfmn, hfml, hfmk, hp⟩ := ih hl' hk' hllt hklt
+    have ⟨n, l, k, hn, hl, hk, hnn', hll', hkk', hp⟩ := ih hl' hk' hllt hklt
+    replace hlf' : p'.fn[fm'[m]].LocalFn fm'[l] := by grind
     have hne : n ≠ m := by grind
-    have hlf := h'.fn_localProvenance
-      (show m < p'.size by lia) hmlt (by lia) (by grind)
-      (show l < p'.size by lia) (by lia) (by simpa [← hfml] using hlf')
+    have hfmm : fm'.Dom m := ⟨by lia, by grind⟩
+    have hfml : fm'.Dom l := ⟨by lia, by grind⟩
+    have hlf := h'.fn_localProvenance hfmm (hmm' ▸ hmlt) hfml hlf'
     simp only [Option.some.injEq, prefix_subst.fn_eq hm, p'] at hlf
     obtain heq | hlf := hlf
     · grind
-    · exact ⟨n, m, k, hn, hm, hk, hfmn, hfmm, hfmk, .step _ _ _ hne ⟨hm, hlf⟩ hp⟩
+    · exact ⟨n, m, k, hn, hm, hk, hnn', hmm', hkk', .step _ _ _ hne ⟨hm, hlf⟩ hp⟩
 
 theorem Program.free_in_fn_of_free_in_subst_of_ge {p : Program} {e : Expr}
     {vm : VarMap p.size} {fm : FunMap p.size} (hvm : vm.Valid fm)
@@ -996,26 +949,27 @@ theorem Program.free_in_fn_of_free_in_subst_of_ge {p : Program} {e : Expr}
   obtain ⟨k', hklt, hlv', hp'⟩ := (free_in_fn_iff hmlt hne').mp hf'
   have hk' : p.size ≤ k' := by grind [prefix_subst.fn_eq]
   have hnlt : n' < p'.size := by grind
-  obtain ⟨n, m, k, hn, hm, hk, hfmn, hfmm, hfmk, hp⟩ :=
+  obtain ⟨n, m, k, hn, hm, hk, hnn', hmm', hkk', hp⟩ :=
     pathWithout_of_pathWithout_in_subst_of_ge hvm hfm hp hvalid ho hn' hm' hk' hnlt hmlt hklt hp'
+  replace hlv' : p'.fn[fm'[k]].LocalVar fm'[n] := by grind
   have hne : n ≠ m := by grind
-  have hlv := h'.fn_localProvenance
-    (show k < p'.size by lia) hklt (by lia) (by grind)
-    (show n < p'.size by lia) (by lia) (by simpa [← hfmn] using hlv')
+  have hfmk : fm'.Dom k := ⟨by lia, by grind⟩
+  have hfmn : fm'.Dom n := ⟨by lia, by grind⟩
+  have hlv := h'.fn_localProvenance hfmk (hkk' ▸ hklt) hfmn hlv'
   rw [prefix_subst.fn_eq hk] at hlv
   simp only [Option.some.injEq, hp.ne_end, false_or] at hlv
-  exact ⟨n, m, hn, hm, hfmn, hfmm, (free_in_fn_iff hm hne).mpr ⟨k, hk, hlv, hp⟩⟩
+  exact ⟨n, m, hn, hm, hnn', hmm', (free_in_fn_iff hm hne).mpr ⟨k, hk, hlv, hp⟩⟩
 
 theorem Expr.free_of_free_in_subst_of_ge {p : Program} {e : Expr}
     {vm : VarMap p.size} {fm : FunMap p.size} (hvm : vm.Valid fm)
     (hfm : fm.Valid) (hp : p.ValidRefs) (hvalid : p.ValidSubst vm fm)
     (ho : e.DeepOriginal p fm) {n' : Nat} (hn' : p.size ≤ n') :
-    let ⟨p', e', fm', h⟩ := e.subst p vm fm
-    let hsize := h.pre.size_le
+    let ⟨p', e', fm', _⟩ := e.subst p vm fm
     e'.Free p' n' → ∃ (n : Nat) (_ : n < p.size),
       fm'[n] = n' ∧ e.Free p n := by
   intro hf
   let p' := (e.subst p vm fm).program
+  let e' := (e.subst p vm fm).expr
   let fm' := (e.subst p vm fm).funMap
   have hvp' : p'.ValidRefs := Program.validRefs_subst hvm hfm hp ho
   have h' : p'.ValidSubst vm.extend fm' :=
@@ -1026,24 +980,27 @@ theorem Expr.free_of_free_in_subst_of_ge {p : Program} {e : Expr}
   obtain ⟨n, hn, heq⟩ := Program.exists_of_ge_in_subst hfm ho hn' hlt
   obtain hlv' | ⟨m', k', hk', hlf', hp', hlv'⟩ := free_iff.mp hf
   · refine ⟨n, hn, heq, free_of_localVar ?_⟩
-    simpa using localProvenance_subst hvm hfm ho (by lia) (by lia) (heq ▸ hlv')
-  · by_cases hm' : m' < p.size
-    · have hk' : k' < p.size := by grind
-      grind [Program.prefix_subst.fn_eq]
+    have hfmn : fm'.Dom n := ⟨by lia, by grind⟩
+    simpa using localProvenance_subst hvm hfm ho hfmn (heq ▸ hlv')
+  · have hklt : k' < p'.size := by grind
+    by_cases hm' : m' < p.size
+    · grind [Program.prefix_subst.fn_eq]
     · simp only [Nat.not_lt] at hm'
       have hk' : p.size ≤ k' := by grind [Program.prefix_subst.fn_eq]
-      obtain ⟨n, m, k, hn, hm, hk, hfmn, hfmm, hfmk, hp⟩ :=
+      obtain ⟨n, m, k, hn, hm, hk, hnn', hmm', hkk', hp⟩ :=
         Program.pathWithout_of_pathWithout_in_subst_of_ge hvm hfm hp hvalid ho hn' hm' hk'
           ‹_› (validRefs_subst hvm hfm ho hlf') ‹_› hp'
-      have hlf := localProvenance_subst hvm hfm ho
-        (show m < p'.size by lia) (by lia) (by simpa [← hfmm] using hlf')
+      replace hlf' : e'.LocalFn fm'[m] := by grind
+      replace hlv' : p'.fn[fm'[k]].LocalVar fm'[n] := by grind
+      have hfmn : fm'.Dom n := ⟨by lia, by grind⟩
+      have hfmm : fm'.Dom m := ⟨by lia, by grind⟩
+      have hfmk : fm'.Dom k := ⟨by lia, by grind⟩
+      have hlf := localProvenance_subst hvm hfm ho hfmm hlf'
       simp only [reduceCtorEq, false_or] at hlf
-      have hlv := h'.fn_localProvenance
-        (show k < p'.size by lia) (show k' < p'.size by grind) (by lia) (by grind)
-        (show n < p'.size by lia) (by lia) (by simpa [← hfmn] using hlv')
+      have hlv := h'.fn_localProvenance hfmk (hkk' ▸ hklt) hfmn hlv'
       rw [Program.prefix_subst.fn_eq hk] at hlv
       simp only [Option.some.injEq, hp.ne_end, false_or] at hlv
-      exact ⟨n, hn, hfmn, free_iff.mpr <| Or.inr ⟨m, k, hk, hlf, hp, hlv⟩⟩
+      exact ⟨n, hn, hnn', free_iff.mpr <| Or.inr ⟨m, k, hk, hlf, hp, hlv⟩⟩
 
 theorem Program.nests_of_nests_in_subst_of_lt {p : Program} {e : Expr}
     {vm : VarMap p.size} {fm : FunMap p.size} {m n : Nat} (hn : n < p.size)
@@ -1056,7 +1013,7 @@ theorem Program.nests_of_nests_in_subst_of_ge {p : Program} {e : Expr}
     (ho : e.DeepOriginal p fm) {n' m' : Nat} (hn' : p.size ≤ n') :
     let ⟨p', _, fm', _⟩ := e.subst p vm fm
     n' ≻[p'] m' → ∃ (n m : Nat) (hn : n < p.size) (hm : m < p.size),
-      fm'[n]'(by grind) = n' ∧ fm'[m]'(by grind) = m' ∧ n ≻[p] m := by
+      fm'[n] = n' ∧ fm'[m] = m' ∧ n ≻[p] m := by
   intro hnests'
   let p' := (e.subst p vm fm).program
   let fm' := (e.subst p vm fm).funMap
@@ -1071,11 +1028,12 @@ theorem Program.nests_of_nests_in_subst_of_ge {p : Program} {e : Expr}
     exact ⟨n, m, hn, hm, hfmn, hfmm, .free _ _ hn hm hne hf⟩
   | trans n' k' m' hnests₁' hnests₂' ih₁ ih₂ =>
     have hk' : p.size ≤ k' := by grind
-    obtain ⟨n, k, hn, hk, hfmn, hfmk, hnests₁⟩ := ih₁ hn'
-    obtain ⟨l, m, hl, hm, hfml, hfmm, hnests₂⟩ := ih₂ hk'
-    obtain rfl : k = l :=
-      hfm'.inj (by grind) (by grind) (by lia) (by lia) (by simp [fm', hfmk, hfml])
-    exact ⟨n, m, hn, hm, hfmn, hfmm, .trans _ _ _ hnests₁ hnests₂⟩
+    obtain ⟨n, k, hn, hk, hnn', hkk', hnests₁⟩ := ih₁ hn'
+    obtain ⟨l, m, hl, hm, hll', hmm', hnests₂⟩ := ih₂ hk'
+    have hfmk : fm'.Dom k := ⟨by grind, by grind⟩
+    have hfml : fm'.Dom l := ⟨by grind, by grind⟩
+    obtain rfl : k = l := hfm'.inj hfmk hfml (by simp [fm', hkk', hll'])
+    exact ⟨n, m, hn, hm, hnn', hmm', .trans _ _ _ hnests₁ hnests₂⟩
 
 theorem Program.subst_wf {p : Program} {e : Expr} {vm : VarMap p.size}
     {fm : FunMap p.size} (hvm : vm.Valid fm) (hfm : fm.Valid) (hp : p.ValidRefs)
@@ -1089,63 +1047,35 @@ theorem Program.subst_wf {p : Program} {e : Expr} {vm : VarMap p.size}
   · simp only [Nat.not_lt] at hm
     have hvalid' : p'.ValidSubst vm.extend fm' := validSubst_subst hvm hfm hp h ho
     have hfm' : fm'.Valid := FunMap.valid_subst hfm ho
-    replace ⟨k, l, hk, hl, hfmk, hfml, hnests⟩ :=
+    replace ⟨k, l, hk, hl, hkk', hll', hnests⟩ :=
       nests_of_nests_in_subst_of_ge hvm hfm hp h ho hm hnests
-    obtain rfl : k = l :=
-      hfm'.inj (by grind) (by grind) (by lia) (by lia) (by simp [fm', hfmk, hfml])
+    have hfmk : fm'.Dom k := ⟨by grind, by grind⟩
+    have hfml : fm'.Dom l := ⟨by grind, by grind⟩
+    obtain rfl : k = l := hfm'.inj hfmk hfml (by simp [fm', hkk', hll'])
     exact hwf hnests
 
 def Expr.WFSubst (e : Expr) (p : Program) (vm : VarMap p.size)
     (fm : FunMap p.size) : Prop :=
-  ∀ ⦃n m⦄ (_ : n < p.size) (_ : m < p.size),
-    n ≻[p] m → e.Free p m → vm[n] ≠ var n → vm[m] ≠ var m ∧ fm[m] ≠ m
+  ∀ ⦃n m⦄, n ≻[p] m → e.Free p m → vm.Dom n → vm.Dom m ∧ fm.Dom m
 
 @[grind =]
 theorem Expr.wfSubst_bin_iff {k : BinKind} {e₁ e₂ : Expr} {p : Program}
     {vm : VarMap p.size} {fm : FunMap p.size} :
     (e₁.bin k e₂).WFSubst p vm fm ↔ e₁.WFSubst p vm fm ∧ e₂.WFSubst p vm fm := by
-  constructor
-  · intro h
-    and_intros
-    · intro n m hn hm hnests hf hne
-      exact h hn hm hnests (.binL _ _ _ hf) hne
-    · intro n m hn hm hnests hf hne
-      exact h hn hm hnests (.binR _ _ _ hf) hne
-  · rintro ⟨h₁, h₂⟩ n m hn hm hnests hf hne
-    cases hf with
-    | binL _ _ _ hf => exact h₁ hn hm hnests hf hne
-    | binR _ _ _ hf => exact h₂ hn hm hnests hf hne
+  grind [WFSubst]
 
 @[grind =]
 theorem Expr.wfSubst_cond_iff {c et ef : Expr} {p : Program} {vm : VarMap p.size}
     {fm : FunMap p.size} :
     (c.cond et ef).WFSubst p vm fm ↔
       c.WFSubst p vm fm ∧ et.WFSubst p vm fm ∧ ef.WFSubst p vm fm := by
-  constructor
-  · intro h
-    and_intros
-    · intro n m hn hm hnests hf hne
-      exact h hn hm hnests (.condC _ _ _ hf) hne
-    · intro n m hn hm hnests hf hne
-      exact h hn hm hnests (.condT _ _ _ hf) hne
-    · intro n m hn hm hnests hf hne
-      exact h hn hm hnests (.condF _ _ _ hf) hne
-  · rintro ⟨h₁, h₂, h₃⟩ n m hn hm hnests hf hne
-    cases hf with
-    | condC _ _ _ hf => exact h₁ hn hm hnests hf hne
-    | condT _ _ _ hf => exact h₂ hn hm hnests hf hne
-    | condF _ _ _ hf => exact h₃ hn hm hnests hf hne
+  grind [WFSubst]
 
 @[grind =]
 theorem Expr.wfSubst_proj_iff {e : Expr} {i : Fin 2} {p : Program}
     {vm : VarMap p.size} {fm : FunMap p.size} :
     (e.proj i).WFSubst p vm fm ↔ e.WFSubst p vm fm := by
-  constructor
-  · intro h n m hn hm hnests hf hne
-    exact h hn hm hnests (.proj _ _ hf) hne
-  · intro h n m hn hm hnests hf hne
-    replace .proj _ _ hf := hf
-    exact h hn hm hnests hf hne
+  grind [WFSubst]
 
 theorem Expr.wfSubst_in_subst {p : Program} {e₁ e₂ : Expr} {vm : VarMap p.size}
     {fm : FunMap p.size} (hfm : fm.Valid) (hp : p.ValidRefs)
@@ -1157,79 +1087,32 @@ theorem Expr.wfSubst_in_subst {p : Program} {e₁ e₂ : Expr} {vm : VarMap p.si
 
 theorem Expr.exists_free_subst_var {p : Program} {e : Expr} {vm : VarMap p.size}
     {fm : FunMap p.size} {n m : Nat} {r : RefKind} (he : e.ValidRefs p)
-    (hwfs : e.WFSubst p vm fm) (hn : n < p.size) (hvmn : vm[n] ≠ var n)
+    (hwfs : e.WFSubst p vm fm) (hvmn : vm.Dom n)
     (hnests : n ≻[p] m) (hl : e.Local m r) :
-    ∃ (k : Nat) (_ : k < p.size), vm[k] ≠ var k ∧ e.Free p k := by
+    ∃ (k : Nat), vm.Dom k ∧ e.Free p k := by
   have hm := he hl
   cases r with
   | var =>
     have hf : e.Free p m := Expr.free_of_localVar hl
-    obtain ⟨hvmm, -⟩ := hwfs hn hm hnests hf hvmn
-    exact ⟨m, hm, hvmm, hf⟩
+    obtain ⟨hvmm, -⟩ := hwfs hnests hf hvmn
+    exact ⟨m, hvmm, hf⟩
   | fn =>
     obtain ⟨_, k, hk, hne, hf, hnests⟩ := Program.nests_iff.mp hnests
     replace hf := free_of_localFn_of_free _ hne hl hf
     cases hnests with
-    | refl _ => exact ⟨n, hn, hvmn, hf⟩
+    | refl _ => exact ⟨n, hvmn, hf⟩
     | nests _ hnests =>
-      obtain ⟨hvmk, -⟩ := hwfs hn hk hnests hf hvmn
-      exact ⟨k, hk, hvmk, hf⟩
-
-theorem FunMap.ne_in_subst {p : Program} {e : Expr} {vm : VarMap p.size}
-    {fm : FunMap p.size} {n m : Nat} {r : RefKind} (hvm : vm.Valid fm)
-    (hfm : fm.Valid) (hp : p.ValidRefs) (ho : e.DeepOriginal p fm)
-    (hwfs : e.WFSubst p vm fm) (hn : n < p.size) (hvmn : vm[n] ≠ .var n)
-    (hl : e.Local m r) (hnests : n ≻[p] m) :
-    let ⟨_, _, fm', _⟩ := e.subst p vm fm
-    (fm'[m]'(by grind)) ≠ m := by
-  have hm : m < p.size := ho.validRefs hl
-  fun_induction Expr.subst
-  next p e vm fm h =>
-    obtain ⟨k, hk, hvmk, hf⟩ :=
-      Expr.exists_free_subst_var ho.validRefs hwfs hn hvmn hnests hl
-    have := h k hk hf
-    contradiction
-  next p vm fm m h =>
-    obtain ⟨rfl, rfl⟩ := Expr.local_var_iff.mp hl
-    obtain ⟨-, hmm'⟩ := hwfs _ hm hnests .var hvmn
-    exact hmm'
-  next p vm fm m hm hfmm m' vm₁ fm₁ p₁ p₂ f' fm₂ h₂ hs₂ p₃ e' hf ih =>
-    obtain ⟨rfl, rfl⟩ := Expr.local_fn_iff.mp hl
-    have hext : fm₂.Extends fm₁ := by grind [valid_update]
-    grind
-  next p vm fm m hm hfmm hf =>
-    dsimp only
-    obtain ⟨rfl, rfl⟩ := Expr.local_fn_iff.mp hl
-    assumption
-  next => grind
-  next => grind
-  next p vm fm k e₁ e₂ p₁ e₁' fm₁ h₁ hs₁ p₂ e₂' fm₂ h₂ hs₂ h ih₁ ih₂ =>
-    rw [hs₁] at ih₁
-    rw [hs₂] at ih₂
-    dsimp only at *
-    have hext : fm₂.Extends fm₁ := by grind
-    grind [Program.validRefs_subst, Expr.wfSubst_in_subst]
-  next p vm fm c et ef p₁ c' fm₁ h₁ hs₁ vm₁ p₂ et' fm₂ h₂ hs₂ p₃ ef' fm₃ h₃ hs₃
-      hf ihc ihet ihef =>
-    rw [hs₁] at ihc
-    rw [hs₂] at ihet
-    rw [hs₃] at ihef
-    dsimp only at *
-    have hext₁ : fm₂.Extends fm₁ := by grind
-    have hext₂ : fm₃.Extends fm₂ := by grind
-    grind [Program.validRefs_subst, Expr.wfSubst_in_subst]
-  next p vm fm e i p' e' fm' h hs hf ih =>
-    rw [hs] at ih
-    grind
+      obtain ⟨hvmk, -⟩ := hwfs hnests hf hvmn
+      exact ⟨k, hvmk, hf⟩
 
 def FunMap.StrongProvenance (p : Program) (fm : FunMap p.size)
     (vm : VarMap p.size) (e e' : Expr) (k : Option Nat) : Prop :=
   ∀ ⦃m' r⦄ (_ : m' < p.size),
     e'.Local m' r →
       ∃ (m : Nat) (_ : m < p.size),
-        fm[m] = m ∧ (∀ k (_ : k < p.size), vm[k] ≠ .var k → k ⊁[p] m) ∧
+        ¬fm.Dom m ∧ (∀ k, vm.Dom k → k ⊁[p] m) ∧
           (e.LocalVar m ∧ vm[m].Local m' r ∨ e.LocalFn m ∧ m' = m ∧ r = .fn) ∨
-          fm[m] = m' ∧ (m = k ∨ e.Local m r ∧ m' ≠ m)
+          fm[m] = m' ∧ (m = k ∨ e.Local m r ∧ fm.Dom m)
 
 theorem FunMap.strongProvenance_bin {p : Program} {vm : VarMap p.size}
     {fm : FunMap p.size} {k : BinKind} {e₁ e₁' e₂ e₂' : Expr}
@@ -1264,44 +1147,45 @@ theorem Expr.strongProvenance_subst {p : Program} {e : Expr}
   fun_induction subst
   next p e vm fm h =>
     intro n r hn hl
-    have hnnests : ∀ m (_ : m < p.size), vm[m] ≠ var m → m ⊁[p] n := by
-      intro m hm hvmm hnests
-      obtain ⟨k, hk, hvmk, hf⟩ :=
-        exists_free_subst_var ho.validRefs hwfe hm hvmm hnests hl
-      have := h k hk hf
+    have hnnests : ∀ m, vm.Dom m → m ⊁[p] n := by
+      intro m hvmm hnests
+      obtain ⟨k, hvmk, hf⟩ :=
+        exists_free_subst_var ho.validRefs hwfe hvmm hnests hl
+      have := h k hf
       contradiction
-    have hfmn := hvalid.eq_of_not_nests hn hnnests
+    have hfmn : ¬fm.Dom n := by
+      intro hfmn
+      obtain ⟨m, hvmm, hnests⟩ := hvalid.nests_of_dom hfmn
+      exact hnnests m hvmm hnests
     refine ⟨n, hn, Or.inl ⟨hfmn, by grind, ?_⟩⟩
     cases r with
     | var =>
-      have hf := h _ hn (free_of_localVar hl)
-      exact Or.inl ⟨hl, by simp [*]⟩
+      have hf := h _ (free_of_localVar hl)
+      exact Or.inl ⟨hl, by simp_all [VarMap.Dom]⟩
     | fn => exact Or.inr ⟨hl, rfl, rfl⟩
-  next p vm fm m h =>
+  next p vm fm m hvmm =>
     intro n r hn hl
-    by_cases hm : m < p.size
-    · simp only [Classical.not_forall] at h
-      obtain ⟨k, hk, hf, hvmk⟩ := h
-      have .var := hf
-      simp only [getElem?_pos, Option.getD_some, hk] at hl
-      by_cases hkk' : fm[k] = k
-      · refine ⟨k, hk, Or.inl ⟨hkk', ?_, Or.inl ⟨.var, by grind⟩⟩⟩
-        intro l hl hvml hnests
-        exact hvmk <| hvalid.new_subst_var hl hk (by grind) hnests hkk'
-      · refine ⟨k, hk, Or.inr ?_⟩
-        cases hvalid.compat hk hkk' <;> grind
-    · simp_all
+    simp only [free_in_var_iff, forall_eq, Classical.not_not] at hvmm
+    have hm := hvmm.1
+    simp only [getElem?_pos, Option.getD_some, hm] at hl
+    by_cases hfmk : fm.Dom m
+    · refine ⟨m, hm, Or.inr ?_⟩
+      have := hvalid.compat hfmk hvmm
+      grind
+    · refine ⟨m, hm, Or.inl ⟨hfmk, ?_, Or.inl ⟨.var, by grind⟩⟩⟩
+      intro l hvml hnests
+      exact hfmk <| hvalid.dom_of_nests (by grind) hnests hvmm
+  next p vm fm m hm hfmm hf =>
+    intro n r hn hl
+    simp only [local_fn_iff] at hl
+    obtain ⟨rfl, rfl⟩ := hl
+    exact ⟨m, hm, Or.inr ⟨rfl, Or.inr ⟨.fn, hfmm⟩⟩⟩
   next p vm fm m hm hfmm m' vm₁ fm₁ p₁ p₂ f' fm₂ h₂ hs₂ p₃ e' hf ih =>
     intro m'' r hm' hl
     simp only [Expr.local_fn_iff, e'] at hl
     obtain ⟨hr, rfl⟩ := hl
     have hext : fm₂.Extends fm₁ := by grind [FunMap.valid_update]
     exact ⟨m, by lia, Or.inr (by grind [hext.eq])⟩
-  next p vm fm m hm hfmm hf =>
-    intro n r hn hl
-    simp only [local_fn_iff] at hl
-    obtain ⟨rfl, rfl⟩ := hl
-    exact ⟨m, hm, Or.inr ⟨rfl, Or.inr ⟨.fn, hfmm⟩⟩⟩
   next p vm fm m hm h =>
     intro m' r hm' hl
     simp only [local_fn_iff] at hl
@@ -1323,10 +1207,9 @@ theorem Expr.strongProvenance_subst {p : Program} {e : Expr}
     replace he₁' : fm₂.StrongProvenance p₂ vm.extend e₁ e₁' none := by
       intro n r hn hl
       replace hn : n < p₁.size := by grind [validRefs_subst]
-      obtain ⟨m, hm, ⟨hmm', hnnests, h⟩ | ⟨hfmm, h | ⟨hl, hor⟩⟩⟩ := he₁' hn hl
-      · refine ⟨m, by grind, Or.inl
-          ⟨hvalid₂.eq_of_not_nests (by grind) ?hf, ?hf, by grind⟩⟩
-        grind
+      obtain ⟨m, hm, ⟨hfmm, hnnests, h⟩ | ⟨hfmm, h | ⟨hl, hor⟩⟩⟩ := he₁' hn hl
+      · replace hfmm : ¬fm₂.Dom m := by grind [hvalid₂.nests_of_dom]
+        exact ⟨m, by grind, Or.inl ⟨hfmm, by grind, by grind⟩⟩
       · contradiction
       · exact ⟨m, by grind, Or.inr ⟨by grind, Or.inr ⟨hl, by grind⟩⟩⟩
     exact FunMap.strongProvenance_bin he₁' he₂'
@@ -1352,19 +1235,17 @@ theorem Expr.strongProvenance_subst {p : Program} {e : Expr}
     replace hc' : fm₃.StrongProvenance p₃ vm.extend c c' none := by
       intro n r hn hl
       replace hn : n < p₁.size := by grind [validRefs_subst]
-      obtain ⟨m, hm, ⟨hmm', hnnests, h⟩ | ⟨hfmm, h | ⟨hl, hor⟩⟩⟩ := hc' hn hl
-      · refine ⟨m, by grind, Or.inl
-          ⟨hvalid₃.eq_of_not_nests (by grind) ?hc, ?hc, by grind⟩⟩
-        grind
+      obtain ⟨m, hm, ⟨hfmm, hnnests, h⟩ | ⟨hfmm, h | ⟨hl, hor⟩⟩⟩ := hc' hn hl
+      · replace hfmm : ¬fm₃.Dom m := by grind [hvalid₃.nests_of_dom]
+        exact ⟨m, by grind, Or.inl ⟨hfmm, by grind, by grind⟩⟩
       · contradiction
       · exact ⟨m, by grind, Or.inr ⟨by grind, Or.inr ⟨hl, by grind⟩⟩⟩
     replace het' : fm₃.StrongProvenance p₃ vm.extend et et' none := by
       intro n r hn hl
       replace hn : n < p₂.size := by grind [validRefs_subst]
-      obtain ⟨m, hm, ⟨hmm', hnnests, h⟩ | ⟨hfmm, h | ⟨hl, hor⟩⟩⟩ := het' hn hl
-      · refine ⟨m, by grind, Or.inl
-          ⟨hvalid₃.eq_of_not_nests (by grind) ?het, ?het, by grind⟩⟩
-        grind
+      obtain ⟨m, hm, ⟨hfmm, hnnests, h⟩ | ⟨hfmm, h | ⟨hl, hor⟩⟩⟩ := het' hn hl
+      · replace hfmm : ¬fm₃.Dom m := by grind [hvalid₃.nests_of_dom]
+        exact ⟨m, by grind, Or.inl ⟨hfmm, by grind, by grind⟩⟩
       · contradiction
       · exact ⟨m, by grind, Or.inr ⟨by grind, Or.inr ⟨hl, by grind⟩⟩⟩
     exact FunMap.strongProvenance_cond hc' het' hef'
@@ -1387,22 +1268,19 @@ theorem Program.push_wf {p : Program} {b : Expr} {t₁ t₂ : Ty} (hp : p.ValidR
 
 def Program.WFSubst (p : Program) (vm : VarMap p.size) (fm : FunMap p.size) :
     Prop :=
-  ∀ ⦃m m'⦄ (_ : m < p.size) (_ : m' < p.size),
-    fm[m] = m' → m' ≠ m → fm.StrongProvenance p vm p.fn[m] p.fn[m'] m
+  ∀ ⦃m⦄ (hm : fm.Dom m) (_ : fm[m] < p.size),
+    fm.StrongProvenance p vm p.fn[m] p.fn[fm[m]] m
 
 theorem Program.wfSubst_fn_mk {p : Program} {n : Nat} {v : Expr}
     (hn : n < p.size) (hwf : p.WF) :
     p.fn[n].WFSubst p (.mk _ n v) (.mk _) := by
-  intro k m hk hm hnests hf hne
-  by_cases n = k
-  · subst k
-    simp only [VarMap.mk, Vector.getElem_setIfInBounds_self, ne_eq] at hne
-    exfalso
-    by_cases h : m = n
-    · subst m
-      exact hwf hnests
-    · exact hwf (nests_iff.mpr ⟨hk, _, hm, h, hf, .nests _ hnests⟩)
-  · simp [VarMap.mk, *] at hne
+  intro k m hnests hf hvmk
+  obtain rfl : n = k := by grind
+  exfalso
+  by_cases h : m = n
+  · subst m
+    exact hwf hnests
+  · exact hwf (nests_iff.mpr ⟨hvmk.1, _, by grind, h, hf, .nests _ hnests⟩)
 
 theorem Program.wfSubst_mk {p : Program} {n : Nat} {v : Expr} :
     p.WFSubst (.mk _ n v) (.mk _) := by
@@ -1410,32 +1288,28 @@ theorem Program.wfSubst_mk {p : Program} {n : Nat} {v : Expr} :
 
 theorem Program.wfSubst_push_recurse {p : Program} {vm : VarMap p.size}
     {fm : FunMap p.size} (hfm : fm.Valid) (hp : p.ValidRefs) {l i : Nat}
-    (hl : l < p.size) (hi : i < p.size) (hvml : vm[l] ≠ .var l)
-    (hfmi : fm[i] = i) (hnestsi : l ≻[p] i)
+    (hi : i < p.size) (hvml : vm.Dom l) (hfmi : ¬fm.Dom i) (hnestsi : l ≻[p] i)
     (hwfs : p.WFSubst vm fm) :
     (p.push (.recurse p.size) p.ty[i] p.ret[i]).WFSubst
       (vm.update i hi) (fm.update i hi) := by
-  intro m m' hm hm' rfl hmm'
+  intro m hfmm hm'
   by_cases m = p.size
-  · simp [*] at hmm'
-  · replace hm : m < p.size := by lia
+  · grind
+  · replace hm : m < p.size := by grind
     by_cases i = m
     · intro n r hn hlc
       grind
     · intro n r hn hlc
       replace hm' : fm[m] < p.size := by grind
-      simp only [ne_eq, not_false_eq_true, FunMap.getElem_update_ne,
-        Vector.getElem_push_lt, *] at hlc hmm'
       replace hn : n < p.size := by grind
       obtain ⟨k, hk, ⟨hvmk, hnnests, hlc⟩ | ⟨hfmk, heq | ⟨hlc, h⟩⟩⟩ :=
-        hwfs hm hm' rfl hmm' hn hlc
+        hwfs (by grind) hm' hn (by simpa [*] using hlc)
       · have : i ≠ k := by grind
-        exact ⟨k, by lia, Or.inl ⟨by simp [*], by grind, by simp [*]⟩⟩
+        exact ⟨k, by lia, Or.inl ⟨by grind, by grind, by simp [*]⟩⟩
       · grind
       · have : i ≠ k := by grind
-        exact ⟨k, by lia, by simp [*]⟩
+        exact ⟨k, by lia, by grind⟩
 
-set_option maxHeartbeats 1000000 in
 theorem Program.wfSubst_subst {p : Program} {e : Expr}
     {vm : VarMap p.size} {fm : FunMap p.size} (hvm : vm.Valid fm) (hfm : fm.Valid)
     (hp : p.ValidRefs) (hvalid : p.ValidSubst vm fm) (hwf : p.WF)
@@ -1447,63 +1321,57 @@ theorem Program.wfSubst_subst {p : Program} {e : Expr}
   next p vm fm m hm hfmm m' vm₁ fm₁ p₁ p₂ f' fm₂ h₂ hs₂ p₃ e' hf ih =>
     rw [hs₂] at ih
     dsimp only at *
-    simp only [Classical.not_forall] at hf
-    obtain ⟨l, hl, hf, hvml⟩ := hf
+    simp only [Classical.not_forall, Classical.not_not] at hf
+    obtain ⟨l, hf, hvml⟩ := hf
     have hnestsm : l ≻[p] m := by
       replace .fn _ hm hne hf := hf
-      exact .free _ _ hl hm hne hf
+      exact .free _ _ hvml.1 hm hne hf
     obtain ⟨hom, hm, ho⟩ := Expr.deepOriginal_fn_iff.mp ho
     have ho' : p.fn[m].DeepOriginal p₁ fm₁ := by grind
     have hvm₁ : vm₁.Valid fm₁ := VarMap.valid_update hm hvm hfm
     have hfm₁ : fm₁.Valid := FunMap.valid_update hm hom hfm
     have hp₁ : p₁.ValidRefs := validRefs_push hp (by grind)
     have hvalid₁ : p₁.ValidSubst vm₁ fm₁ :=
-      validSubst_push_recurse hl hm hfm hp hvml hnestsm hvalid
+      validSubst_push_recurse hm hfm hp hvml hnestsm hvalid
     have hwf₁ : p₁.WF := push_wf hp hwf
     have hwfs₁ : p₁.WFSubst vm₁ fm₁ :=
-      wfSubst_push_recurse hfm hp hl hm hvml hfmm hnestsm hwfs
+      wfSubst_push_recurse hfm hp hm hvml hfmm hnestsm hwfs
     have hwfsm : p.fn[m].WFSubst p₁ vm₁ fm₁ := by
-      intro n k hn hk hnests hf hne
+      intro n k hnests hf hvmn
       by_cases m = k
-      · simp only [VarMap.getElem_update_eq, ne_eq, Expr.var.injEq, FunMap.getElem_update_eq,
-          and_self, vm₁, fm₁, *]
-        lia
-      · replace hn : n < p.size := by grind
-        simp only [ne_eq, vm₁] at hne ⊢
+      · grind
+      · have hn : n < p.size := by grind
+        replace hfmm : fm₁.Dom m := by grind
         replace hnests : n ≻[p] k := by grind
         replace hf : p.fn[m].Free p k := by grind
-        replace hk : k < p.size :=
-          Expr.lt_size_of_free hp (hp hm) hf
-        rw [VarMap.getElem_update_ne hm hk ‹_›]
+        replace hk : k < p.size := Expr.lt_size_of_free hp (hp hm) hf
         have hmn : m ≠ n := by
           intro rfl
           exfalso
           exact hwf (nests_iff.mpr ⟨hm, _, hk, ‹m ≠ k›.symm, hf, .nests _ hnests⟩)
-        simp only [ne_eq, not_false_eq_true, VarMap.getElem_update_ne, hn, hmn] at hne
-        have := hwfe hn hk hnests (.fn _ hm ‹m ≠ k›.symm hf) hne
-        simp [fm₁, *]
+        grind [hwfe hnests (.fn _ hm ‹m ≠ k›.symm hf) (by grind)]
     have hwfs₂ := ih hvm₁ hfm₁ hp₁ hvalid₁ hwf₁ ho' hwfs₁ hwfsm
     have hext₂ : fm₂.Extends fm₁ := by grind
     have hfm₂ : fm₂.Valid := hext₂.valid
-    have hfmm : fm₂[m]'(by grind) = m' := by grind [hext₂.eq]
-    have hfmm' : fm₂[m']'(by grind) = m' := by grind
-    have hp₃ : p₃ = ((Expr.fn m).subst p vm fm).program := by
-      grind [Expr.subst]
+    have hmm' : fm₂[m] = m' := by grind [hext₂.eq]
+    have hfmm' : fm₂[m'] = m' := by grind
     have hpre₂ : p.Prefix p₂ := prefix_trans prefix_push h₂.pre
-    have hpre₃ : p.Prefix p₃ := hp₃ ▸ prefix_subst
-    intro n n' hn hn' rfl hnn'
+    have hpre₃ : p.Prefix p₃ := by grind
+    intro n hfmn hn'
     replace hn : n < p.size := by
       false_or_by_contra
       have hn' : p₁.size ≤ n := by grind
       obtain ⟨k, hk, hfmk⟩ :=
-        exists_of_ge_in_subst (e := p.fn[m]) (vm := vm₁) hfm₁ ho' hn' (by lia)
+        exists_of_ge_in_subst (vm := vm₁) hfm₁ ho' hn' (by grind)
       have hp₂ : p₂ = (p.fn[m].subst p₁ vm₁ fm₁).program := by grind
       subst p₂
-      grind [hfm₂.idem]
+      have hfm₂ : fm₂ = (p.fn[m].subst p₁ vm₁ fm₁).funMap := by grind
+      subst fm₂
+      exact hfm₂.not_dom_map (by grind) (hfmk ▸ hfmn)
     by_cases m = n
     · subst n
       simp only [ne_eq, show m' ≠ m by lia, not_false_eq_true, Vector.getElem_set_ne,
-        Vector.getElem_set_self, p₃, hfmm]
+        Vector.getElem_set_self, p₃, hmm']
       have hf' := Expr.strongProvenance_subst hvm₁ hfm₁ hp₁ hvalid₁ hwf₁ ho' hwfsm
       rw [hs₂] at hf'
       dsimp only at hf'
@@ -1513,24 +1381,18 @@ theorem Program.wfSubst_subst {p : Program} {e : Expr}
       · have hl : l < p.size := by grind
         by_cases m = l
         · exact ⟨m, by lia, Or.inr (by grind)⟩
-        · exact ⟨l, hl', Or.inl ⟨hll', by
-            intro k hk hvmk
-            simp only [p₃] at hpre₃
-            simp [nests_in_prefix_iff hl hp hpre₂] at hnnests
-            rw [nests_in_prefix_iff hl hp hpre₃]
-            exact hnnests k hk (by grind),
-            by grind⟩⟩
+        · exact ⟨l, hl', Or.inl ⟨hll', by grind, by grind⟩⟩
       · contradiction
       · exact ⟨l, hl', Or.inr ⟨hfml, Or.inr ⟨hlc, h⟩⟩⟩
     · have : m' ≠ n := by grind
       have : m' ≠ fm₂[n] := by
         intro h
-        have := hfm₂.inj (show m < p₂.size by lia) (by lia) (by lia) hnn' (hfmm ▸ h)
+        have := hfm₂.inj (by grind) hfmn (hmm' ▸ h)
         contradiction
       simp only [ne_eq, not_false_eq_true, Vector.getElem_set_ne, p₃, *]
       intro k r hk hlc
       obtain ⟨l, hl, ⟨hmm', hnnests, h⟩ | ⟨hfml, h | ⟨hlc, h⟩⟩⟩ :=
-        hwfs₂ (by lia) (by lia) rfl hnn' hk hlc
+        hwfs₂ hfmn (by lia) hk hlc
       · by_cases m = l
         · exact ⟨m, by lia, Or.inr (by grind)⟩
         · have : vm₁.extend[l] = vm.extend[l] := by
@@ -1542,12 +1404,7 @@ theorem Program.wfSubst_subst {p : Program} {e : Expr}
               · simp [*]
               · simp [show p.size + 1 ≤ l by lia, *]
           rw [this] at h
-          refine ⟨l, hl, Or.inl ⟨hmm', ?_, h⟩⟩
-          rw [show p₂.fn[n] = p.fn[n] by grind] at h
-          replace hl : l < p.size := by grind
-          intro o ho hvmo hnests
-          replace hnests : o ≻[p₂] l := by grind
-          exact hnnests o ho (by grind) hnests
+          exact ⟨l, hl, Or.inl ⟨hmm', by grind, h⟩⟩
       · grind
       · grind
   next p vm fm k e₁ e₂ p₁ e₁' fm₁ h₁ hs₁ p₂ e₂' fm₂ h₂ hs₂ h ih₁ ih₂ =>
@@ -1561,16 +1418,14 @@ theorem Program.free_in_fn_of_free_in_subst {p : Program} {e : Expr}
     {vm : VarMap p.size} {fm : FunMap p.size} (hvm : vm.Valid fm)
     (hfm : fm.Valid) (hp : p.ValidRefs) (hvalid : p.ValidSubst vm fm)
     (hwf : p.WF) (hwfs : p.WFSubst vm fm) (ho : e.DeepOriginal p fm)
-    (hwfe : e.WFSubst p vm fm) {n' m m' : Nat} (hm : m < p.size) :
-    let ⟨p', _, fm', h⟩ := e.subst p vm fm
-    let hsize := h.pre.size_le
-    ∀ (_ : m' < p'.size), fm'[m] = m' → m' ≠ m → n' ≠ m' → p'.fn[m'].Free p' n' →
-      ∃ (n : Nat) (hn : n < p.size), p.fn[m].Free p n ∧
-          (fm'[n] = n ∧ vm[n].Free p n' ∨ fm'[n] = n' ∧ n' ≠ n) := by
-  intro hm' hfmm hmm' hne hf
+    (hwfe : e.WFSubst p vm fm) {n' m : Nat} (hm : m < p.size) :
+    let (eq := hs) ⟨p', _, fm', _⟩ := e.subst p vm fm
+    fm'.Dom m → n' ≠ fm'[m] → p'.fn[fm'[m]].Free p' n' →
+      ∃ (n : Nat) (hf : p.fn[m].Free p n),
+          (¬fm'.Dom n ∧ vm[n].Free p n' ∨ fm'[n] = n' ∧ fm'.Dom n) := by
+  intro hfmm hne hf
   let p' := (e.subst p vm fm).program
   let fm' := (e.subst p vm fm).funMap
-  let hsize := (e.subst p vm fm).props.pre.size_le
   have hfm' : fm'.Valid := FunMap.valid_subst hfm ho
   have hp' : p'.ValidRefs := validRefs_subst hvm hfm hp ho
   have hvalid' : p'.ValidSubst vm.extend fm' :=
@@ -1578,27 +1433,29 @@ theorem Program.free_in_fn_of_free_in_subst {p : Program} {e : Expr}
   have hwfs' : p'.WFSubst vm.extend fm' :=
     wfSubst_subst hvm hfm hp hvalid hwf ho hwfs hwfe
   obtain ⟨k', hk', hlv, hpath⟩ := (free_in_fn_iff _ hne).mp hf
+  generalize hmm' : fm'[m] = m' at hpath
   induction hpath generalizing m with
   | refl m' hne =>
     have hn' : n' < p'.size := by grind
+    replace hlv : p'.fn[fm'[m]].LocalVar n' := by grind
     obtain ⟨n, hn, ⟨hnn', hvmn, ⟨hlv, hlc⟩ | h⟩ | ⟨hfmn, h | ⟨hlc, hnn'⟩⟩⟩ :=
-      hwfs' (by lia) hm' hfmm hmm' hn' hlv
+      hwfs' hfmm (by grind) hn' hlv
     · rw [prefix_subst.fn_eq hm] at hlv
       replace hn : n < p.size := hp hm hlv
       simp only [hn, VarMap.getElem_extend_lt] at hlc
-      exact ⟨n, hn, Expr.free_of_localVar hlv,
+      exact ⟨n, Expr.free_of_localVar hlv,
         Or.inl ⟨hnn', Expr.free_of_localVar hlc⟩⟩
     · grind
     · grind
     · rw [prefix_subst.fn_eq hm] at hlc
       replace hn : n < p.size := hp hm hlc
-      exact ⟨n, hn, Expr.free_of_localVar hlc, Or.inr ⟨hfmn, hnn'⟩⟩
+      exact ⟨n, Expr.free_of_localVar hlc, Or.inr ⟨hfmn, hnn'⟩⟩
   | step m' l' k' hne hs hpath ih =>
-    have hmm' : m' ≠ m := by lia
     obtain ⟨_, hlf⟩ := hs
     have hl' : l' < p'.size := by grind
-    obtain ⟨l, hl, ⟨hll', hnnests, ⟨hlvm, hlf⟩ | ⟨hlf, rfl, -⟩⟩ | ⟨hfml, h | ⟨hlf, hll'⟩⟩⟩ :=
-      hwfs' (by lia) hm' hfmm hmm' hl' hlf
+    replace hlf : p'.fn[fm'[m]].LocalFn l' := by grind
+    obtain ⟨l, hl, ⟨hll', hnnests, ⟨hlvm, hlf⟩ | ⟨hlf, rfl, -⟩⟩ | ⟨rfl, h | ⟨hlf, hfml⟩⟩⟩ :=
+      hwfs' hfmm (by grind) hl' hlf
     · replace hl : l < p.size := by grind
       replace hlf : vm[l].LocalFn l' := by grind
       replace hl' : l' < p.size := by grind
@@ -1606,17 +1463,17 @@ theorem Program.free_in_fn_of_free_in_subst {p : Program} {e : Expr}
       replace hpath : l' ⟶[p, n']* k' := by grind
       rw [prefix_subst.fn_eq hm] at hlvm
       rw [prefix_subst.fn_eq hk'] at hlv
-      exact ⟨l, hl, Expr.free_of_localVar hlvm,
+      exact ⟨l, Expr.free_of_localVar hlvm,
         Or.inl ⟨hll', Expr.free_iff.mpr (Or.inr ⟨l', k', hk', hlf, hpath, hlv⟩)⟩⟩
     · replace hl' : l' < p.size := by grind
       replace hk' : k' < p.size := by grind
       have hn' : n' < p.size := by grind
       have hne := hpath.ne_start
-      have hnn' : fm'[n'] = n' := by
-        apply hvalid'.eq_of_not_nests
-        intro n hn hvmn hnests
-        refine hnnests n hn hvmn
-          (.trans _ _ _ hnests (.free _ _ (by lia) (by lia) hne ?_))
+      have hfmn : ¬fm'.Dom n' := by
+        intro hfmn
+        obtain ⟨n, hvmn, hnests⟩ := hvalid'.nests_of_dom hfmn
+        refine hnnests n hvmn
+          (.trans _ _ _ hnests (.free _ _ (by grind) (by lia) hne ?_))
         exact (free_in_fn_iff (by lia) hne).mpr ⟨_, ‹_›, hlv, hpath⟩
       replace hpath : l' ⟶[p, n']* k' := by grind
       rw [prefix_subst.fn_eq hm] at hlf
@@ -1627,16 +1484,17 @@ theorem Program.free_in_fn_of_free_in_subst {p : Program} {e : Expr}
       have hvmn' : vm[n'] = .var n' := by
         false_or_by_contra
         rename_i hvmn'
-        grind [Nests.free]
-      exact ⟨n', hn', free_in_fn_of_succ hl' hne ⟨hm, hlf⟩ hf,
-        Or.inl ⟨hnn', hvmn' ▸ .var⟩⟩
+        replace hvmn' : vm.Dom n' := ⟨_, hvmn'⟩
+        grind [Nests.free _ _ hn' hl' hne hf]
+      exact ⟨n', free_in_fn_of_succ hl' hne ⟨hm, hlf⟩ hf,
+        Or.inl ⟨hfmn, hvmn' ▸ .var⟩⟩
     · grind
     · rw [prefix_subst.fn_eq hm] at hlf
       replace hl : l < p.size := by grind
       replace hne := hpath.ne_start
       replace hf := (free_in_fn_iff hl' hne).mpr ⟨k', hk', hlv, hpath⟩
-      obtain ⟨n, hn, hf, h⟩ := ih hl hl' hfml hll' hne hf hk' hlv
-      exact ⟨n, hn, free_in_fn_of_succ hl (by grind) ⟨hm, hlf⟩ hf, h⟩
+      obtain ⟨n, hf, h⟩ := ih hl hfml hne hf hk' hlv rfl
+      exact ⟨n, free_in_fn_of_succ hl (by grind) ⟨hm, hlf⟩ hf, h⟩
 
 theorem Expr.free_of_free_in_subst {p : Program} {e : Expr} {vm : VarMap p.size}
     {fm : FunMap p.size} (hvm : vm.Valid fm) (hfm : fm.Valid) (hp : p.ValidRefs)
@@ -1644,56 +1502,55 @@ theorem Expr.free_of_free_in_subst {p : Program} {e : Expr} {vm : VarMap p.size}
     (ho : e.DeepOriginal p fm) (hwfe : e.WFSubst p vm fm)
     {n' : Nat} :
     let ⟨p', e', fm', h⟩ := e.subst p vm fm
-    let hsize := h.pre.size_le
-    e'.Free p' n' → ∃ (n : Nat) (hn : n < p.size), e.Free p n ∧
-      (fm'[n] = n ∧ vm[n].Free p n' ∨ fm'[n] = n' ∧ n' ≠ n) := by
+    e'.Free p' n' → ∃ (n : Nat) (hf : e.Free p n),
+      (¬fm'.Dom n ∧ vm[n].Free p n' ∨ fm'[n] = n' ∧ fm'.Dom n) := by
   intro hf
   let p' := (e.subst p vm fm).program
   let e' := (e.subst p vm fm).expr
   let fm' := (e.subst p vm fm).funMap
-  let hsize := (e.subst p vm fm).props.pre.size_le
   have hfm' : fm'.Valid := FunMap.valid_subst hfm ho
   have hvalid' : p'.ValidSubst vm.extend fm' :=
     Program.validSubst_subst hvm hfm hp hvalid ho
   have he' : e'.ValidRefs p' := validRefs_subst hvm hfm ho
   obtain hlv | ⟨m', k', hk', hlf, hpath, hlv⟩ := free_iff.mp hf
   · have hn' : n' < p'.size := by grind
-    obtain ⟨n, hn, ⟨hnn', hnnests, ⟨hlv, hl⟩ | ⟨-, -, h⟩⟩ | ⟨hfmn, h | ⟨hlv, hnn'⟩⟩⟩ :=
+    obtain ⟨n, hn, ⟨hfmn, hnnests, ⟨hlv, hl⟩ | ⟨-, -, h⟩⟩ | ⟨hfmn, h | ⟨hlv, hnn'⟩⟩⟩ :=
       strongProvenance_subst hvm hfm hp hvalid hwf ho hwfe hn' hlv
-    · exact ⟨n, ho.validRefs hlv, free_of_localVar hlv,
-        Or.inl ⟨hnn', free_of_localVar (by grind)⟩⟩
+    · exact ⟨n, free_of_localVar hlv,
+        Or.inl ⟨hfmn, free_of_localVar (by grind)⟩⟩
     · contradiction
     · contradiction
-    · exact ⟨n, ho.validRefs hlv, free_of_localVar hlv, Or.inr ⟨hfmn, hnn'⟩⟩
+    · exact ⟨n, free_of_localVar hlv, Or.inr ⟨hfmn, hnn'⟩⟩
   · have hm' : m' < p'.size := by grind
     have hne := hpath.ne_start
     replace hf' := (Program.free_in_fn_iff hm' hne).mpr ⟨_, hk', hlv, hpath⟩
-    obtain ⟨m, hm, ⟨hmm', hnnests, h⟩ | ⟨hfmm, h | ⟨hlf, hmm'⟩⟩⟩ :=
+    obtain ⟨m, hm, ⟨hfmm, hnnests, h⟩ | ⟨rfl, h | ⟨hlf, hmm'⟩⟩⟩ :=
       strongProvenance_subst hvm hfm hp hvalid hwf ho hwfe hm' hlf
     · replace hm : m < p.size := by grind
       replace hm' : m' < p.size := by grind
       obtain ⟨hlv, hlc⟩ | ⟨hlf, rfl, -⟩ := h
-      · refine ⟨m, hm, free_of_localVar hlv, Or.inl ⟨hmm', ?_⟩⟩
+      · refine ⟨m, free_of_localVar hlv, Or.inl ⟨hfmm, ?_⟩⟩
         exact free_of_localFn_of_free hm' hne (by grind) (by grind)
       · have hn' : n' < p.size := by grind
-        have hnn' : fm'[n'] = n' := by
-          apply hvalid'.eq_of_not_nests
-          intro n hn hvmn hnests
-          refine hnnests n hn hvmn
-            (.trans _ _ _ hnests (.free _ _ (by lia) (by lia) hne ?_))
+        have hfmn : ¬fm'.Dom n' := by
+          intro hfmn
+          obtain ⟨n, hvmn, hnests⟩ := hvalid'.nests_of_dom hfmn
+          refine hnnests n hvmn
+            (.trans _ _ _ hnests (.free _ _ (by grind) (by lia) hne ?_))
           exact (Program.free_in_fn_iff (by lia) hne).mpr ⟨_, ‹_›, hlv, hpath⟩
         have hvmn' : vm[n'] = .var n' := by
           false_or_by_contra
           rename_i hvmn'
-          exact hnnests n' (by lia) (by grind) (.free _ _ (by lia) (by lia) hne hf')
-        exact ⟨n', hn', free_of_localFn_of_free hm' hne hlf (by grind),
-          Or.inl ⟨hnn', hvmn' ▸ Free.var⟩⟩
+          replace hvmn' : vm.Dom n' := ⟨hn', hvmn'⟩
+          exact hnnests n' (by grind) (.free _ _ (by grind) (by lia) hne hf')
+        exact ⟨n', free_of_localFn_of_free hm' hne hlf (by grind),
+          Or.inl ⟨hfmn, hvmn' ▸ Free.var⟩⟩
     · contradiction
     · replace hm : m < p.size := by grind
-      obtain ⟨n, hn, hf, h⟩ :=
+      obtain ⟨n, hf, h⟩ :=
         Program.free_in_fn_of_free_in_subst hvm hfm hp hvalid hwf hwfs ho hwfe
-        hm hm' hfmm hmm' hne hf'
-      exact ⟨n, hn, free_of_localFn_of_free hm (by grind) hlf hf, h⟩
+        hm hmm' hne hf'
+      exact ⟨n, free_of_localFn_of_free hm (by grind) hlf hf, h⟩
 
 public section
 
@@ -1716,32 +1573,29 @@ theorem Computation.free_of_free_in_subst {c : Computation} {n m : Nat}
     | refl _ => exact hwf hnests
     | nests _ h => exact hwf (.trans _ _ _ hnests h)
   have hwfs : e.WFSubst p vm fm := by
-    intro k l hk hl hnests hf h
+    intro k l hnests hf h
     have : n ≠ k := by
       intro rfl
       exact hnnests _ hf hnests
-    simp [VarMap.mk, vm, *] at h
+    grind
   let p' := (e.subst p vm fm).program
   let fm' := (e.subst p vm fm).funMap
-  let hsize := (e.subst p vm fm).props.pre.size_le
   have hvalid' : p'.ValidSubst vm.extend fm' :=
     Program.validSubst_subst hvm hfm hp hvalid ho
-  obtain ⟨k, hk, hf, ⟨hkk', hf'⟩ | ⟨hfmk, hne⟩⟩ :=
+  obtain ⟨k, hf, ⟨hkk', hf'⟩ | ⟨hfmk, hne⟩⟩ :=
     Expr.free_of_free_in_subst hvm hfm hp hvalid hwf Program.wfSubst_mk ho hwfs hf
   · by_cases n = k
     · subst k
       simp only [VarMap.mk, Vector.getElem_setIfInBounds_self, vm] at hf'
       exact Or.inr hf'
-    · simp [VarMap.mk, vm, *] at hf'
-      have .var := hf'
-      exact Or.inl ⟨hf, ‹n ≠ m›.symm⟩
-  · have hkk' : fm'[k] = k := by
-      apply hvalid'.eq_of_not_nests
-      intro l hl hvml hnests
-      obtain rfl : n = l := by grind
+    · simp only [VarMap.mk, ne_eq, not_false_eq_true, Vector.getElem_setIfInBounds_ne,
+        Vector.getElem_ofFn, Expr.free_in_var_iff, vm, *] at hf'
+      exact Or.inl ⟨hf' ▸ hf, hf' ▸ ‹n ≠ k›.symm⟩
+  · have hfmk : ¬fm'.Dom k := by
+      intro hfmk
+      obtain ⟨l, hvml, hnests⟩ := hvalid'.nests_of_dom hfmk
       replace hnests : n ≻[p] k := by grind
       exact hnnests _ hf hnests
-    rw [hfmk] at hkk'
     contradiction
 
 theorem Computation.subst_types {c : Computation} {t : Ty} {n : Nat} {v : Expr}
